\begin{loigiaibt}{6}
  Ta có $A=[-2;2]$ và $B=(-\infty ;1)$, suy ra \begin {itemize} \item $A\cup B=[-2;2]\cup (-\infty ;1)=(-\infty ;2]$. \item $A\cap B=[-2;2]\cap (-\infty ;1)=[-2;1)$. \item $A\setminus B=[-2;2]\setminus (-\infty ;1)=[1;2]$. \item $C_{\mathbb {R}}B=[1;+\infty )$. \end {itemize}  
\end{loigiaibt}
\begin{loigiaibt}{7}
  \begin {multicols}{2} \begin {enumerate} \item $ A=\{x \in \mathbb {N^*} | x<10\} $. \item $ D=\{2^n | n \in \mathbb {N}, n \le 9 \} $. \item $ E=\{2n | n \in \mathbb {Z}\} $. \item $ F=\{2n+1 | n \in \mathbb {Z}\} $. \end {enumerate} \end {multicols}  
\end{loigiaibt}
\begin{loigiaibt}{8}
  \begin {enumerate} \item $A=\left \{M\in (P)\big | OM=R \text { với } O \text { cố định cho trước}\right \}$. \item $B=\left \{M\in (P)\big | OM\leqslant R\text { với } O \text { cố định cho trước}\right \}$. \end {enumerate}  
\end{loigiaibt}
